Foundation/ProvabilityLogic/GLBeta/Basic.lean
@@ -17,12 +17,12 @@ namespace FFL.ProvabilityLogic
 
 open Formula LetterlessFormula
 
-/-- The letterless formula `∼⋀_{n ∉ X} TBB n` for a cofinite `X`. -/
-noncomputable def LetterlessFormula.betaMinus (X : Set ℕ) (hX : Xᶜ.Finite) : LetterlessFormula :=
-  ∼(⩕ n ∈ hX.toFinset, TBB n)
+/-- The formula `∼⋀_{n ∉ X} alpha n` for a cofinite `X`. -/
+noncomputable def Formula.beta {α : Type*} (X : Set ℕ) (hX : Xᶜ.Finite) : Formula α :=
+  ∼(⩕ n ∈ hX.toFinset, alpha n)
 
 noncomputable abbrev Logic.GLBeta {α : Type*} (X : Set ℕ) (hX : Xᶜ.Finite) : Logic α :=
-  𝐆𝐋 +ᴸ {(betaMinus X hX).lift}
+  𝐆𝐋 +ᴸ {beta X hX}
 
 notation "𝐆𝐋β" => Logic.GLBeta
 
@@ -30,19 +30,22 @@ variable {α : Type*} {X : Set ℕ} {hX : Xᶜ.Finite}
 
 namespace LetterlessFormula
 
-@[simp]
-lemma spectrum_betaMinus : spectrum (betaMinus X hX) = Xᶜ := by
-  ext n;
-  simp [betaMinus];
+@[simp, grind =] lemma lift_beta : lift (beta X hX) = (beta X hX : Formula α) := by
+  simp [beta, lift_neg, lift_conj'];
 
 @[simp]
-lemma trace_betaMinus : trace (betaMinus X hX) = X := by
+lemma spectrum_beta : spectrum (beta X hX) = Xᶜ := by
+  ext n;
+  simp [beta];
+
+@[simp]
+lemma trace_beta : trace (beta X hX) = X := by
   simp [trace];
 
 end LetterlessFormula
 
 lemma Logic.GLBeta.eq_sumQuasiNormal_lift :
-    (𝐆𝐋β X hX : Logic α) = (𝐆𝐋 +ᴸ LetterlessFormulaSet.lift {betaMinus X hX}) := by
+    (𝐆𝐋β X hX : Logic α) = (𝐆𝐋 +ᴸ LetterlessFormulaSet.lift {beta X hX}) := by
   simp;
 
 end FFL.ProvabilityLogic
